Source/DafnyCore/DafnyPrelude.bpl
@@ -201,7 +201,7 @@ axiom (forall bx : Box, t : Ty ::
     ( $IsBox(bx, TMultiSet(t)) ==> $Box($Unbox(bx) : MultiSet Box) == bx && $Is($Unbox(bx) : MultiSet Box, TMultiSet(t))));
 axiom (forall bx : Box, t : Ty ::
     { $IsBox(bx, TSeq(t)) }
-    ( $IsBox(bx, TSeq(t)) ==> $Box($Unbox(bx) : Seq Box) == bx && $Is($Unbox(bx) : Seq Box, TSeq(t))));
+    ( $IsBox(bx, TSeq(t)) ==> $Box($Unbox(bx) : Seq) == bx && $Is($Unbox(bx) : Seq, TSeq(t))));
 axiom (forall bx : Box, s : Ty, t : Ty ::
     { $IsBox(bx, TMap(s, t)) }
     ( $IsBox(bx, TMap(s, t)) ==> $Box($Unbox(bx) : Map Box Box) == bx && $Is($Unbox(bx) : Map Box Box, TMap(s, t))));
@@ -247,7 +247,7 @@ axiom (forall v: MultiSet Box, t0: Ty :: { $Is(v, TMultiSet(t0)) }
     0 < v[bx] ==> $IsBox(bx, t0)));
 axiom (forall v: MultiSet Box, t0: Ty :: { $Is(v, TMultiSet(t0)) }
   $Is(v, TMultiSet(t0)) ==> $IsGoodMultiSet(v));
-axiom (forall v: Seq Box, t0: Ty :: { $Is(v, TSeq(t0)) }
+axiom (forall v: Seq, t0: Ty :: { $Is(v, TSeq(t0)) }
   $Is(v, TSeq(t0)) <==>
   (forall i : int :: { Seq#Index(v, i) }
     0 <= i && i < Seq#Length(v) ==>
@@ -304,7 +304,7 @@ axiom (forall v: MultiSet Box, t0: Ty, h: Heap :: { $IsAlloc(v, TMultiSet(t0), h
   $IsAlloc(v, TMultiSet(t0), h) <==>
   (forall bx: Box :: { v[bx] }
     0 < v[bx] ==> $IsAllocBox(bx, t0, h)));
-axiom (forall v: Seq Box, t0: Ty, h: Heap :: { $IsAlloc(v, TSeq(t0), h) }
+axiom (forall v: Seq, t0: Ty, h: Heap :: { $IsAlloc(v, TSeq(t0), h) }
   $IsAlloc(v, TSeq(t0), h) <==>
   (forall i : int :: { Seq#Index(v, i) }
     0 <= i && i < Seq#Length(v) ==>
@@ -921,51 +921,51 @@ axiom (forall<T> s: Set T :: { MultiSet#Card(MultiSet#FromSet(s)) }
   MultiSet#Card(MultiSet#FromSet(s)) == Set#Card(s));
 
 // conversion to a multiset, from a sequence.
-function MultiSet#FromSeq(Seq Box): MultiSet Box uses {
-  axiom MultiSet#FromSeq(Seq#Empty(): Seq Box) == MultiSet#Empty(): MultiSet Box;
+function MultiSet#FromSeq(Seq): MultiSet Box uses {
+  axiom MultiSet#FromSeq(Seq#Empty(): Seq) == MultiSet#Empty(): MultiSet Box;
 }
 
 // conversion produces a good map.
-axiom (forall s: Seq Box :: { MultiSet#FromSeq(s) } $IsGoodMultiSet(MultiSet#FromSeq(s)) );
+axiom (forall s: Seq :: { MultiSet#FromSeq(s) } $IsGoodMultiSet(MultiSet#FromSeq(s)) );
 // cardinality axiom
-axiom (forall s: Seq Box ::
+axiom (forall s: Seq ::
   { MultiSet#Card(MultiSet#FromSeq(s)) }
     MultiSet#Card(MultiSet#FromSeq(s)) == Seq#Length(s));
 // building axiom
-axiom (forall s: Seq Box, v: Box ::
+axiom (forall s: Seq, v: Box ::
   { MultiSet#FromSeq(Seq#Build(s, v)) }
     MultiSet#FromSeq(Seq#Build(s, v)) == MultiSet#UnionOne(MultiSet#FromSeq(s), v)
   );
 
 // concatenation axiom
-axiom (forall a: Seq Box, b: Seq Box ::
+axiom (forall a: Seq, b: Seq ::
   { MultiSet#FromSeq(Seq#Append(a, b)) }
     MultiSet#FromSeq(Seq#Append(a, b)) == MultiSet#Union(MultiSet#FromSeq(a), MultiSet#FromSeq(b)) );
 
 // update axiom
-axiom (forall s: Seq Box, i: int, v: Box, x: Box ::
+axiom (forall s: Seq, i: int, v: Box, x: Box ::
   { MultiSet#FromSeq(Seq#Update(s, i, v))[x] }
     0 <= i && i < Seq#Length(s) ==>
     MultiSet#FromSeq(Seq#Update(s, i, v))[x] ==
       MultiSet#Union(MultiSet#Difference(MultiSet#FromSeq(s), MultiSet#Singleton(Seq#Index(s,i))), MultiSet#Singleton(v))[x] );
   // i.e. MS(Update(s, i, v)) == MS(s) - {{s[i]}} + {{v}}
-axiom (forall s: Seq Box, x: Box :: { MultiSet#FromSeq(s)[x] }
+axiom (forall s: Seq, x: Box :: { MultiSet#FromSeq(s)[x] }
   (exists i : int :: { Seq#Index(s,i) } 0 <= i && i < Seq#Length(s) && x == Seq#Index(s,i)) <==> 0 < MultiSet#FromSeq(s)[x] );
 
 // ---------------------------------------------------------------
 // -- Axiomatization of sequences --------------------------------
 // ---------------------------------------------------------------
 
-type Seq T;
+type Seq;
 
-function Seq#Length(Seq Box): int;
-axiom (forall s: Seq Box :: { Seq#Length(s) } 0 <= Seq#Length(s));
+function Seq#Length(Seq): int;
+axiom (forall s: Seq :: { Seq#Length(s) } 0 <= Seq#Length(s));
 
-function Seq#Empty(): Seq Box uses {
-  axiom Seq#Length(Seq#Empty(): Seq Box) == 0;
+function Seq#Empty(): Seq uses {
+  axiom Seq#Length(Seq#Empty(): Seq) == 0;
 }
 
-axiom (forall s: Seq Box :: { Seq#Length(s) }
+axiom (forall s: Seq :: { Seq#Length(s) }
   (Seq#Length(s) == 0 ==> s == Seq#Empty())
 // The following would be a nice fact to include, because it would enable verifying the
 // GenericPick.SeqPick* methods in Test/dafny0/SmallTests.dfy.  However, it substantially
@@ -975,126 +975,126 @@ axiom (forall s: Seq Box :: { Seq#Length(s) }
   );
 
 // The empty sequence $Is any type
-//axiom (forall t: Ty :: {$Is(Seq#Empty(): Seq Box, TSeq(t))} $Is(Seq#Empty(): Seq Box, TSeq(t)));
+//axiom (forall t: Ty :: {$Is(Seq#Empty(): Seq, TSeq(t))} $Is(Seq#Empty(): Seq, TSeq(t)));
 
-function Seq#Singleton(Box): Seq Box;
+function Seq#Singleton(Box): Seq;
 axiom (forall t: Box :: { Seq#Length(Seq#Singleton(t)) } Seq#Length(Seq#Singleton(t)) == 1);
 
-function Seq#Build(s: Seq Box, val: Box): Seq Box;
-function Seq#Build_inv0(s: Seq Box) : Seq Box;
-function Seq#Build_inv1(s: Seq Box) : Box;
-axiom (forall s: Seq Box, val: Box ::
+function Seq#Build(s: Seq, val: Box): Seq;
+function Seq#Build_inv0(s: Seq) : Seq;
+function Seq#Build_inv1(s: Seq) : Box;
+axiom (forall s: Seq, val: Box ::
   { Seq#Build(s, val) }
   Seq#Build_inv0(Seq#Build(s, val)) == s &&
   Seq#Build_inv1(Seq#Build(s, val)) == val);
 
-axiom (forall s: Seq Box, v: Box ::
+axiom (forall s: Seq, v: Box ::
   { Seq#Build(s,v) }
   Seq#Length(Seq#Build(s,v)) == 1 + Seq#Length(s));
-axiom (forall s: Seq Box, i: int, v: Box :: { Seq#Index(Seq#Build(s,v), i) }
+axiom (forall s: Seq, i: int, v: Box :: { Seq#Index(Seq#Build(s,v), i) }
   (i == Seq#Length(s) ==> Seq#Index(Seq#Build(s,v), i) == v) &&
   (i != Seq#Length(s) ==> Seq#Index(Seq#Build(s,v), i) == Seq#Index(s, i)));
 
 // Build preserves $Is
-axiom (forall s: Seq Box, bx: Box, t: Ty :: { $Is(Seq#Build(s,bx),TSeq(t)) }
+axiom (forall s: Seq, bx: Box, t: Ty :: { $Is(Seq#Build(s,bx),TSeq(t)) }
     $Is(s,TSeq(t)) && $IsBox(bx,t) ==> $Is(Seq#Build(s,bx),TSeq(t)));
 
-function Seq#Create(ty: Ty, heap: Heap, len: int, init: HandleType): Seq Box;
+function Seq#Create(ty: Ty, heap: Heap, len: int, init: HandleType): Seq;
 axiom (forall ty: Ty, heap: Heap, len: int, init: HandleType ::
-  { Seq#Length(Seq#Create(ty, heap, len, init): Seq Box) }
+  { Seq#Length(Seq#Create(ty, heap, len, init): Seq) }
   $IsGoodHeap(heap) && 0 <= len ==>
-  Seq#Length(Seq#Create(ty, heap, len, init): Seq Box) == len);
+  Seq#Length(Seq#Create(ty, heap, len, init): Seq) == len);
 axiom (forall ty: Ty, heap: Heap, len: int, init: HandleType, i: int ::
   { Seq#Index(Seq#Create(ty, heap, len, init), i) }
   $IsGoodHeap(heap) && 0 <= i && i < len ==>
   Seq#Index(Seq#Create(ty, heap, len, init), i) == Apply1(TInt, ty, heap, init, $Box(i)));
 
-function Seq#Append(Seq Box, Seq Box): Seq Box;
-axiom (forall s0: Seq Box, s1: Seq Box :: { Seq#Length(Seq#Append(s0,s1)) }
+function Seq#Append(Seq, Seq): Seq;
+axiom (forall s0: Seq, s1: Seq :: { Seq#Length(Seq#Append(s0,s1)) }
   Seq#Length(Seq#Append(s0,s1)) == Seq#Length(s0) + Seq#Length(s1));
 
-function Seq#Index(Seq Box, int): Box;
+function Seq#Index(Seq, int): Box;
 axiom (forall t: Box :: { Seq#Index(Seq#Singleton(t), 0) } Seq#Index(Seq#Singleton(t), 0) == t);
-axiom (forall s0: Seq Box, s1: Seq Box, n: int :: { Seq#Index(Seq#Append(s0,s1), n) }
+axiom (forall s0: Seq, s1: Seq, n: int :: { Seq#Index(Seq#Append(s0,s1), n) }
   (n < Seq#Length(s0) ==> Seq#Index(Seq#Append(s0,s1), n) == Seq#Index(s0, n)) &&
   (Seq#Length(s0) <= n ==> Seq#Index(Seq#Append(s0,s1), n) == Seq#Index(s1, n - Seq#Length(s0))));
 
-function Seq#Update(Seq Box, int, Box): Seq Box;
-axiom (forall s: Seq Box, i: int, v: Box :: { Seq#Length(Seq#Update(s,i,v)) }
+function Seq#Update(Seq, int, Box): Seq;
+axiom (forall s: Seq, i: int, v: Box :: { Seq#Length(Seq#Update(s,i,v)) }
   0 <= i && i < Seq#Length(s) ==> Seq#Length(Seq#Update(s,i,v)) == Seq#Length(s));
-axiom (forall s: Seq Box, i: int, v: Box, n: int :: { Seq#Index(Seq#Update(s,i,v),n) }
+axiom (forall s: Seq, i: int, v: Box, n: int :: { Seq#Index(Seq#Update(s,i,v),n) }
   0 <= n && n < Seq#Length(s) ==>
     (i == n ==> Seq#Index(Seq#Update(s,i,v),n) == v) &&
     (i != n ==> Seq#Index(Seq#Update(s,i,v),n) == Seq#Index(s,n)));
 
-function Seq#Contains(Seq Box, Box): bool;
-axiom (forall s: Seq Box, x: Box :: { Seq#Contains(s,x) }
+function Seq#Contains(Seq, Box): bool;
+axiom (forall s: Seq, x: Box :: { Seq#Contains(s,x) }
   Seq#Contains(s,x) <==>
     (exists i: int :: { Seq#Index(s,i) } 0 <= i && i < Seq#Length(s) && Seq#Index(s,i) == x));
 axiom (forall x: Box ::
   { Seq#Contains(Seq#Empty(), x) }
   !Seq#Contains(Seq#Empty(), x));
 
-axiom (forall s0: Seq Box, s1: Seq Box, x: Box ::
+axiom (forall s0: Seq, s1: Seq, x: Box ::
   { Seq#Contains(Seq#Append(s0, s1), x) }
   Seq#Contains(Seq#Append(s0, s1), x) <==>
     Seq#Contains(s0, x) || Seq#Contains(s1, x));
 
-axiom (forall s: Seq Box, v: Box, x: Box ::  // needed to prove things like '4 in [2,3,4]', see method TestSequences0 in SmallTests.dfy
+axiom (forall s: Seq, v: Box, x: Box ::  // needed to prove things like '4 in [2,3,4]', see method TestSequences0 in SmallTests.dfy
   { Seq#Contains(Seq#Build(s, v), x) }
     Seq#Contains(Seq#Build(s, v), x) <==> (v == x || Seq#Contains(s, x)));
 
-axiom (forall s: Seq Box, n: int, x: Box ::
+axiom (forall s: Seq, n: int, x: Box ::
   { Seq#Contains(Seq#Take(s, n), x) }
   Seq#Contains(Seq#Take(s, n), x) <==>
     (exists i: int :: { Seq#Index(s, i) }
       0 <= i && i < n && i < Seq#Length(s) && Seq#Index(s, i) == x));
-axiom (forall s: Seq Box, n: int, x: Box ::
+axiom (forall s: Seq, n: int, x: Box ::
   { Seq#Contains(Seq#Drop(s, n), x) }
   Seq#Contains(Seq#Drop(s, n), x) <==>
     (exists i: int :: { Seq#Index(s, i) }
       0 <= n && n <= i && i < Seq#Length(s) && Seq#Index(s, i) == x));
 
-function Seq#Equal(Seq Box, Seq Box): bool;
-axiom (forall s0: Seq Box, s1: Seq Box :: { Seq#Equal(s0,s1) }
+function Seq#Equal(Seq, Seq): bool;
+axiom (forall s0: Seq, s1: Seq :: { Seq#Equal(s0,s1) }
   Seq#Equal(s0,s1) <==>
     Seq#Length(s0) == Seq#Length(s1) &&
     (forall j: int :: { Seq#Index(s0,j) } { Seq#Index(s1,j) }
         0 <= j && j < Seq#Length(s0) ==> Seq#Index(s0,j) == Seq#Index(s1,j)));
-axiom (forall a: Seq Box, b: Seq Box :: { Seq#Equal(a,b) }  // extensionality axiom for sequences
+axiom (forall a: Seq, b: Seq :: { Seq#Equal(a,b) }  // extensionality axiom for sequences
   Seq#Equal(a,b) ==> a == b);
 
-function Seq#SameUntil(Seq Box, Seq Box, int): bool;
-axiom (forall s0: Seq Box, s1: Seq Box, n: int :: { Seq#SameUntil(s0,s1,n) }
+function Seq#SameUntil(Seq, Seq, int): bool;
+axiom (forall s0: Seq, s1: Seq, n: int :: { Seq#SameUntil(s0,s1,n) }
   Seq#SameUntil(s0,s1,n) <==>
     (forall j: int :: { Seq#Index(s0,j) } { Seq#Index(s1,j) }
         0 <= j && j < n ==> Seq#Index(s0,j) == Seq#Index(s1,j)));
 
-function Seq#Take(s: Seq Box, howMany: int): Seq Box;
-axiom (forall s: Seq Box, n: int :: { Seq#Length(Seq#Take(s,n)) }
+function Seq#Take(s: Seq, howMany: int): Seq;
+axiom (forall s: Seq, n: int :: { Seq#Length(Seq#Take(s,n)) }
   0 <= n && n <= Seq#Length(s) ==> Seq#Length(Seq#Take(s,n)) == n);
-axiom (forall s: Seq Box, n: int, j: int ::
+axiom (forall s: Seq, n: int, j: int ::
   {:weight 25}
   { Seq#Index(Seq#Take(s,n), j) }
   { Seq#Index(s, j), Seq#Take(s,n) }
   0 <= j && j < n && j < Seq#Length(s) ==>
     Seq#Index(Seq#Take(s,n), j) == Seq#Index(s, j));
 
-function Seq#Drop(s: Seq Box, howMany: int): Seq Box;
-axiom (forall s: Seq Box, n: int :: { Seq#Length(Seq#Drop(s,n)) }
+function Seq#Drop(s: Seq, howMany: int): Seq;
+axiom (forall s: Seq, n: int :: { Seq#Length(Seq#Drop(s,n)) }
   0 <= n && n <= Seq#Length(s) ==> Seq#Length(Seq#Drop(s,n)) == Seq#Length(s) - n);
-axiom (forall s: Seq Box, n: int, j: int ::
+axiom (forall s: Seq, n: int, j: int ::
   {:weight 25}
   { Seq#Index(Seq#Drop(s,n), j) }
   0 <= n && 0 <= j && j < Seq#Length(s)-n ==>
     Seq#Index(Seq#Drop(s,n), j) == Seq#Index(s, j+n));
-axiom (forall s: Seq Box, n: int, k: int ::
+axiom (forall s: Seq, n: int, k: int ::
   {:weight 25}
   { Seq#Index(s, k), Seq#Drop(s,n) }
   0 <= n && n <= k && k < Seq#Length(s) ==>
     Seq#Index(Seq#Drop(s,n), k-n) == Seq#Index(s, k));
 
-axiom (forall s, t: Seq Box, n: int ::
+axiom (forall s, t: Seq, n: int ::
   { Seq#Take(Seq#Append(s, t), n) }
   { Seq#Drop(Seq#Append(s, t), n) }
   n == Seq#Length(s)
@@ -1102,7 +1102,7 @@ axiom (forall s, t: Seq Box, n: int ::
   Seq#Take(Seq#Append(s, t), n) == s &&
   Seq#Drop(Seq#Append(s, t), n) == t);
 
-function Seq#FromArray(h: Heap, a: ref): Seq Box;
+function Seq#FromArray(h: Heap, a: ref): Seq;
 axiom (forall h: Heap, a: ref ::
   { Seq#Length(Seq#FromArray(h,a)) }
   Seq#Length(Seq#FromArray(h, a)) == _System.array.Length(a));
@@ -1113,7 +1113,7 @@ axiom (forall h: Heap, a: ref ::
     // the relation between the array and the sequence can be proved in either
     // direction
     { read(h, a, IndexField(i)) }
-    { Seq#Index(Seq#FromArray(h, a): Seq Box, i) }
+    { Seq#Index(Seq#FromArray(h, a): Seq, i) }
     0 <= i &&
     i < Seq#Length(Seq#FromArray(h, a))  // this will trigger the previous axiom to get a connection with _System.array.Length(a)
     ==>
@@ -1128,16 +1128,16 @@ axiom (forall h: Heap, i: int, v: Box, a: ref ::
     0 <= i && i < _System.array.Length(a) ==> Seq#FromArray(update(h, a, IndexField(i), v), a) == Seq#Update(Seq#FromArray(h, a), i, v) );
 
 // Commutability of Take and Drop with Update.
-axiom (forall s: Seq Box, i: int, v: Box, n: int ::
+axiom (forall s: Seq, i: int, v: Box, n: int ::
         { Seq#Take(Seq#Update(s, i, v), n) }
         0 <= i && i < n && n <= Seq#Length(s) ==> Seq#Take(Seq#Update(s, i, v), n) == Seq#Update(Seq#Take(s, n), i, v) );
-axiom (forall s: Seq Box, i: int, v: Box, n: int ::
+axiom (forall s: Seq, i: int, v: Box, n: int ::
         { Seq#Take(Seq#Update(s, i, v), n) }
         n <= i && i < Seq#Length(s) ==> Seq#Take(Seq#Update(s, i, v), n) == Seq#Take(s, n));
-axiom (forall s: Seq Box, i: int, v: Box, n: int ::
+axiom (forall s: Seq, i: int, v: Box, n: int ::
         { Seq#Drop(Seq#Update(s, i, v), n) }
         0 <= n && n <= i && i < Seq#Length(s) ==> Seq#Drop(Seq#Update(s, i, v), n) == Seq#Update(Seq#Drop(s, n), i-n, v) );
-axiom (forall s: Seq Box, i: int, v: Box, n: int ::
+axiom (forall s: Seq, i: int, v: Box, n: int ::
         { Seq#Drop(Seq#Update(s, i, v), n) }
         0 <= i && i < n && n <= Seq#Length(s) ==> Seq#Drop(Seq#Update(s, i, v), n) == Seq#Drop(s, n));
 // Extension axiom, triggers only on Takes from arrays.
@@ -1145,30 +1145,30 @@ axiom (forall h: Heap, a: ref, n0, n1: int ::
         { Seq#Take(Seq#FromArray(h, a), n0), Seq#Take(Seq#FromArray(h, a), n1) }
         n0 + 1 == n1 && 0 <= n0 && n1 <= _System.array.Length(a) ==> Seq#Take(Seq#FromArray(h, a), n1) == Seq#Build(Seq#Take(Seq#FromArray(h, a), n0), read(h, a, IndexField(n0): Field Box)) );
 // drop commutes with build.
-axiom (forall s: Seq Box, v: Box, n: int ::
+axiom (forall s: Seq, v: Box, n: int ::
         { Seq#Drop(Seq#Build(s, v), n) }
         0 <= n && n <= Seq#Length(s) ==> Seq#Drop(Seq#Build(s, v), n) == Seq#Build(Seq#Drop(s, n), v) );
 
-function Seq#Rank(Seq Box): int;
-axiom (forall s: Seq Box, i: int ::
+function Seq#Rank(Seq): int;
+axiom (forall s: Seq, i: int ::
         { DtRank($Unbox(Seq#Index(s, i)): DatatypeType) }
         0 <= i && i < Seq#Length(s) ==> DtRank($Unbox(Seq#Index(s, i)): DatatypeType) < Seq#Rank(s) );
-axiom (forall s: Seq Box, i: int ::
+axiom (forall s: Seq, i: int ::
         { Seq#Rank(Seq#Drop(s, i)) }
         0 < i && i <= Seq#Length(s) ==> Seq#Rank(Seq#Drop(s, i)) < Seq#Rank(s) );
-axiom (forall s: Seq Box, i: int ::
+axiom (forall s: Seq, i: int ::
         { Seq#Rank(Seq#Take(s, i)) }
         0 <= i && i < Seq#Length(s) ==> Seq#Rank(Seq#Take(s, i)) < Seq#Rank(s) );
-axiom (forall s: Seq Box, i: int, j: int ::
+axiom (forall s: Seq, i: int, j: int ::
         { Seq#Rank(Seq#Append(Seq#Take(s, i), Seq#Drop(s, j))) }
         0 <= i && i < j && j <= Seq#Length(s) ==> Seq#Rank(Seq#Append(Seq#Take(s, i), Seq#Drop(s, j))) < Seq#Rank(s) );
 
 // Additional axioms about common things
-axiom (forall s: Seq Box, n: int :: { Seq#Drop(s, n) }
+axiom (forall s: Seq, n: int :: { Seq#Drop(s, n) }
         n == 0 ==> Seq#Drop(s, n) == s);
-axiom (forall s: Seq Box, n: int :: { Seq#Take(s, n) }
+axiom (forall s: Seq, n: int :: { Seq#Take(s, n) }
         n == 0 ==> Seq#Take(s, n) == Seq#Empty());
-axiom (forall s: Seq Box, m, n: int :: { Seq#Drop(Seq#Drop(s, m), n) }
+axiom (forall s: Seq, m, n: int :: { Seq#Drop(Seq#Drop(s, m), n) }
         0 <= m && 0 <= n && m+n <= Seq#Length(s) ==>
         Seq#Drop(Seq#Drop(s, m), n) == Seq#Drop(s, m+n));
 
